work on repeat toy examples: add inductive PathIn

Pdl/Repeat.lean
@@ -1,6 +1,7 @@
 import Std.Data.List.Lemmas
 import Aesop
 import Mathlib.Tactic.Tauto
+import Mathlib.Tactic.Convert
 
 -- This file is not part of PDL, but just a playground for
 -- representing trees with repeats / back-pointers.
@@ -21,13 +22,12 @@ inductive Tree
 -- * DEFINITIONS
 
 inductive Step : Nat → List Nat → Type
-| up    : Step k     [k+1]
-| down  : Step (k+2) [k]
-| split j k : Step (j+k) [j,k]
+| up    : Step k     [k+2]
+| split : Step (k+1) [1,k]
 
-inductive HisTree : (List Nat) → Nat → Type
-| leaf : HisTree H 0
-| step : Step n ms → (∀ {m}, m ∈ ms → HisTree (n :: H) m) → HisTree H n
+inductive HisTree : List Nat → Nat → Type
+| leaf : HisTree H 1
+| step : {ms : _} → Step n ms → (∀ {m}, m ∈ ms → HisTree (n :: H) m) → HisTree H n
 | rep : m ∈ H → HisTree H m
 
 open Step HisTree
@@ -37,16 +37,7 @@ def helper (t : HisTree H j) (m_def : m ∈ [j]) : HisTree H m :=
 
 -- * EXAMPLES
 
-example : HisTree [] 4 :=
-  -- 4
-  step down $ helper $
-  -- 2
-  step down $ helper
-  -- 0
-  leaf
-
-
-def helperSplit (m_def : m ∈ [j1, j2]) (t1 : HisTree H j1) (t2 : HisTree H j2) : (HisTree H m) :=
+def helperSplit (t1 : HisTree H j1) (t2 : HisTree H j2) (m_def : m ∈ [j1, j2]) : (HisTree H m) :=
   if h1 : m = j1 then
     h1 ▸ t1
   else if h2 : m = j2 then
@@ -54,33 +45,90 @@ def helperSplit (m_def : m ∈ [j1, j2]) (t1 : HisTree H j1) (t2 : HisTree H j2)
   else
     by exfalso; aesop
 
-example : HisTree [] 4 :=
-  --   4
-  step (split 2 2) $
-  -- 2   2
-  (fun m_in =>
-    let two_to_zero := (step down $ helper $ leaf)
-  -- 0   0
-    helperSplit m_in
-    two_to_zero
-    two_to_zero)
-
-example : HisTree [] 4 :=
+def bla : HisTree [] 4 :=
   --      4
-  step (split 1 3) $
-  --    1   3
-  (fun m_in =>
-    helperSplit m_in
-    (step up $ helper $
-     -- 2
-     step down $ helper $
-     -- 0
-     leaf)
-           (step up $
-           -- 4 ( repeat)
-           helper $ rep $
-           by aesop)
-  )
+  step split $ helperSplit
+    -- 1    3
+    leaf $
+    step split $ helperSplit
+    --    1   2
+      leaf
+      --      4
+      (step up $ helper $ rep (by aesop))
+
+-- * NEW: PATHS, inductively and hopefully better than the unsafe verson below
+
+inductive PathIn : (Σ H n, HisTree H n) → Type
+| nil : PathIn ht
+| cons m (m_in : m ∈ ms) (rest : PathIn ⟨n :: H, m, next m_in⟩) : PathIn ⟨H, n, step s next⟩
+
+def PathIn.toList : PathIn ⟨H, m, ht⟩ → List Nat
+| nil => []
+| cons m _ rest => m :: toList rest
+
+def treeAt : PathIn ⟨H, n, ht⟩ → (Σ H n, HisTree H n)
+| PathIn.nil => ⟨H, n, ht⟩
+| PathIn.cons _ _ rest => treeAt rest -- wow, that is much simpler than treeAt' :-)
+
+def isPrefixOf : PathIn ⟨H, n, ht⟩ → PathIn ⟨H, n, ht⟩ → Prop
+| PathIn.nil, _ => true
+| PathIn.cons m _ rest, PathIn.cons m' _ rest' => (meq : m = m') → isPrefixOf rest (meq.symm ▸ rest')
+| PathIn.cons _ _ _, PathIn.nil => false
+
+-- Example of a statement about repeats that should be tricky to prove now:
+-- Any path to a repeat must have a prefix to a split.
+-- (This may or may not be similar enough to condition 6a for PDL.)
+theorem rep_needs_split_above
+    (p : PathIn ⟨[], m, ht⟩)
+    (p_is_rep : treeAt p = ⟨Hp, mp, rep k_in⟩)
+  : ∃ (k : Nat) (Hp' : List Nat) (next : _) (p' : PathIn ⟨[], m, ht⟩),
+      isPrefixOf p' p ∧ (treeAt p' = ⟨Hp', k+1, step (@split k) next⟩) :=
+  by
+  sorry
+
+
+-- TODO: define loopy-paths succ relation including steps via back-loops
+
+
+-- TODO: theorem that there is always a loopy-path to a leaf!?
+
+
+
+-- * OLD: POINTERS AND PATHS, naively - unsafe and safe but (probably) annoyinf to use version
+
+def unsafePointer := (Σ H n, HisTree H n) × List Nat
+
+example : unsafePointer := ⟨⟨_,_,bla⟩, [4,1,(2:Nat)]⟩
+
+def isPathIn : (Σ H n, HisTree H n) → List Nat → Bool
+| _, [] => True
+| ⟨_, k, _⟩, [n]          => n == k
+| ⟨_, 1, leaf⟩,  (_::_::_   ) => False
+| ⟨_, k, rep _, ⟩, (n::_::_   ) => n == k
+| ⟨_, k, @step _ _ ms _ next⟩, (n::m::rest) => n == k ∧ ∃ m_in : m ∈ ms, (isPathIn ⟨_, _, next m_in⟩ (m::rest) )
+
+def SafePathIn (t : Σ H n, HisTree H n) := Subtype (fun l => isPathIn t l)
+
+-- Given a SafePathIn, treeAt' should always return some something, never none.
+
+def treeAt' : List Nat → (Σ H n, HisTree H n) → Option (Σ H n, HisTree H n)
+| [], t => t
+| [n], ⟨H, k, t⟩ => if n == k then some ⟨H,k,t⟩ else none
+| (_::_::_   ), ⟨_, 1,leaf⟩ => none
+| (n::_::_   ), ⟨H, k, rep r⟩ => if n == k then some ⟨H,k, rep r⟩ else none
+| (n::m::rest), ⟨_, k, @step _ _ ms _ next⟩ =>
+  if n == k then
+    if m_in : m ∈ ms then
+      treeAt' (m::rest) ⟨_, _, next m_in⟩
+    else
+      none
+  else
+    none
+
+-- Now, given a SafePathIn leading to a repeat, how do we move back up to the companion?
+-- May need the assumption that H = [], or at least that it is at least as long as the companion-repeat path.
+
+def Pointer := (Σ H n, HisTree H n) × List Nat
 
 -- * CLAIMS
 
